

Q1(a) Let n be an integer. Suppose that n isn't divisible by 5. There is an integer q such that $n = 5q, 5q+1, 5q+2, 5q+3$ or $5q+4$

Since n isn't divisible by 5, the first case isn't possible. We look at $n^4 - 1 = (n^2 + 1)(n^2 - 1) = (n^2 + 1)(n+1)(n-1)$

Case 1 $n = 5q+1$: Then $n^4 - 1 = (n^2 + 1)(n+1)(5q+1-1)$
 $= 5q(n^2 + 1)(n+1)$

Case 2 $n = 5q+2$: Then $n^4 - 1 = ((5q+2)^2 + 1)(n+1)(n-1)$
 $= (25q^2 + 20q + 4 + 1)(n+1)(n-1)$
 $= 5(5q^2 + 4q + 1)(n+1)(n-1)$

Case 3 $n = 5q+3$: Then $n^4 - 1 = ((5q+3)^2 + 1)(n+1)(n-1)$
 $= (25q^2 + 30q + 9 + 1)(n+1)(n-1)$
 $= 5(5q^2 + 6q + 2)(n+1)(n-1)$

Case 4 $n = 5q+4$: Then $n^4 - 1 = (n^2 + 1)(5q+4+1)(n-1)$
 $= 5(q+1)(n^2 + 1)(n-1)$

In all cases, $n^4 - 1$ is divisible by 5.

(2)

Q1(b) Let $a, b, d > 1$ be integers.

Suppose that $a \equiv b \pmod{d}$. Then $d \mid (b-a)$

So there is some integer k such that $k \cdot d = b-a$

$$\text{Then } kd(b+a) = (b-a)(b+a) = b^2 - a^2$$

$$\text{Therefore, } d \mid (b^2 - a^2)$$

$$\text{Thus, } a^2 \equiv b^2 \pmod{d}.$$

Q1(c) They are logically equivalent.

$$\begin{aligned} (p \rightarrow q) \rightarrow (p \wedge r) &\equiv \neg(p \rightarrow q) \vee (p \wedge r) \\ &\equiv \neg(\neg p \vee q) \vee (p \wedge r) \\ &\equiv (\neg\neg p \wedge \neg q) \vee (p \wedge r) \\ &\equiv (p \wedge \neg q) \vee (p \wedge r) \\ &\equiv p \wedge (\neg q \vee r) \\ &\equiv p \wedge (q \rightarrow r) \end{aligned}$$

(Conditional rule)

(Conditional rule)

(De Morgan's Law)

(Double Negation Law)

(Distributive Law)

(Conditional rule)

You may also prove it using a truth table.

(3)

Q2(a)Let n, m be distinct positive integers.Then $n \geq 1$ and $m \geq 1$.Case 1: $n=1$. Then since $n \neq m$, we have $m \geq 2$.

$$\text{Thus } \frac{1}{n} + \frac{1}{m} = \frac{1}{1} + \frac{1}{m} \leq 1 + \frac{1}{2} = \frac{3}{2}.$$

$$\text{and since } \frac{1}{m} > 0, \text{ we also have } \frac{1}{n} + \frac{1}{m} = 1 + \frac{1}{m} > 1$$

$$\text{Thus } 1 < \frac{1}{n} + \frac{1}{m} \leq \frac{3}{2}, \text{ hence } \frac{1}{n} + \frac{1}{m} \text{ is not an integer.}$$

Case 2: $m=1$: Then we argue exactly same as Case 1.Case 3: $n=2$: If $m=1$ then we apply Case 2. Since $n \neq m$,
we have $m \neq 2$. So we assume $m \geq 3$.

$$\text{Then we have } \frac{1}{n} + \frac{1}{m} = \frac{1}{2} + \frac{1}{m} \leq \frac{1}{2} + \frac{1}{3} = \frac{5}{6}$$

$$\text{So } 0 < \frac{1}{n} + \frac{1}{m} \leq \frac{5}{6}, \text{ hence } \frac{1}{n} + \frac{1}{m} \text{ is not an integer.}$$

Case 4: $m=2$: We argue similar to Case 3.Case 5: $n \neq 1$ & $n \neq 2$ & $m \neq 1$ & $m \neq 2$: Then $n \geq 3$ and

$$m \geq 3. \text{ Thus } \frac{1}{n} + \frac{1}{m} \leq \frac{1}{3} + \frac{1}{3} = \frac{2}{3}.$$

$$\text{Since } 0 < \frac{1}{n} + \frac{1}{m} \leq \frac{2}{3}, \text{ hence } \frac{1}{n} + \frac{1}{m} \text{ is not an integer.}$$

In all cases, $\frac{1}{n} + \frac{1}{m}$ is not an integer.

Q2(b)

This is false. Take any number which is both a perfect square and a perfect cube larger than 1. Eg, $a = 64$.

Then a is a perfect square ($a = 8^2$)

but $\sqrt[3]{a} = 4$ is rational.

Q2(c)

This is false. Let $D = \emptyset$, and $E = \{0\}$

are both finite sets, and E has one more element than D .

However, $P(D) = \{\emptyset\}$ and

$P(E) = \{\emptyset, \{0\}\}$

and $P(E)$ has only one more element than $P(D)$.

Q3(a) Let $P(n) : \sum_{j=1}^{3n} j(j-1) = n(9n^2 - 1)$

(5)

Base case : $P(1)$ LHS = $\sum_{j=1}^3 j(j-1) = 1 \cdot 0 + 2 \cdot 1 + 3 \cdot 2$
 $= 0 + 2 + 6$
 $= 8$

RHS = $1 \cdot (9 \cdot 1 - 1) = 8$

So $P(1)$ is true.

Now assume $P(k)$ is true, i.e. $\sum_{j=1}^{3k} j(j-1) = k(9k^2 - 1)$.

Check $P(k+1)$:

$$\sum_{j=1}^{3(k+1)} j(j-1) = \sum_{j=1}^{3k+3} j(j-1) = \sum_{j=1}^{3k} j(j-1) + (3k+1)(3k) + (3k+2)(3k+1) + (3k+3)(3k+2)$$

$$\begin{aligned} &= k(9k^2 - 1) + (3k+1)(3k) + (3k+2)[3k+1 + 3k+3] \\ &= k(3k+1)(3k-1) + (3k+1)(3k) + (3k+2)(6k+4) \\ &= k(3k+1)[3k-1 + 3] + 2(3k+2)^2 \\ &= k(3k+1)(3k+2) + 2(3k+2)^2 \\ &= (3k+2)[k(3k+1) + 2(3k+2)] \\ &= (3k+2)[3k^2 + k + 6k + 4] \\ &= (3k+2)[3k^2 + 7k + 4] \\ &= (3k+2)(k+1)(3k+4) \\ &= (k+1)[(3k+3+1)(3k+3-1)] \\ &= (k+1)[(3k+3)^2 - 1] \\ &= (k+1)[9(k+1)^2 - 1] = \text{RHS.} \end{aligned}$$

Q3(b)

6

Let $P(n)$: for every sequence x_1, x_2, \dots, x_n
of non negative real numbers, if $x_1 + x_2 + \dots + x_n = 0$
then $x_1 = x_2 = \dots = x_n = 0$.

Base case : $P(1)$. We need to check every
non negative real number x_1 .

If $x_1 = 0$ then $x_1 = 0$ is true.

Assume $P(k)$ is true, i.e. for every sequence x_1, x_2, \dots, x_k
of non negative real numbers, if $x_1 + x_2 + \dots + x_k = 0$
then $x_1 = x_2 = \dots = x_k = 0$.

Note that $P(k)$ is a conditional statement !

Now verify $P(k+1)$. Fix a sequence $x_1, x_2, \dots, x_k, x_{k+1}$
of non negative real numbers, and assume that

$$x_1 + x_2 + \dots + x_k + x_{k+1} = 0.$$

$$\text{Then } x_1 + x_2 + \dots + x_k = -x_{k+1}.$$

$$\text{Since } x_{k+1} \geq 0, \text{ hence, RHS} \leq 0.$$

$$\text{Since } x_1 \geq 0, x_2 \geq 0, \dots, x_k \geq 0,$$

$$\text{hence, LHS} \geq 0.$$

But $\text{LHS} = \text{RHS}$, therefore both sides must be 0.

$$\text{So, } x_1 + x_2 + \dots + x_k = -x_{k+1} = 0. \quad \text{—————} (*)$$

From $P(k)$, we know/
assumed $x_1 + x_2 + \dots + x_k = 0 \Rightarrow x_1 = x_2 = \dots = x_k = 0$.

(7)

We also know $x_1 + x_2 + \dots + x_k = 0$ from (*)

So therefore, we conclude $x_1 = x_2 = \dots = x_k = 0$.

From (*) we also know $-x_{k+1} = 0$, so $x_{k+1} = 0$.

Therefore, $x_1 = x_2 = \dots = x_k = x_{k+1} = 0$.

We have shown that starting from $x_1 + x_2 + \dots + x_k + x_{k+1} = 0$

we derived $x_1 = x_2 = \dots = x_k = x_{k+1} = 0$.

So, $P(k+1)$ is true.

Q4(a) Let X and Y be sets.

Let $A \in \mathcal{P}(X-Y) - \{\emptyset\}$.

Thus, $A \in \mathcal{P}(X-Y)$ & $A \notin \{\emptyset\}$.

By definition of powerset, A is not an element of set $\{\emptyset\}$
 this means $A \subseteq X-Y$. So $A \neq \emptyset$.

Since $A \subseteq X-Y$ and $X-Y \subseteq X$

Thus $A \subseteq X$, and so $A \in \mathcal{P}(X)$.

Since $A \neq \emptyset$,

A has some element $a \in A$. Since $A \subseteq X-Y$, it

means $a \in X$ & $a \notin Y$. So, $A \not\subseteq Y$, so $A \notin \mathcal{P}(Y)$.

We conclude $A \in \mathcal{P}(X) - \mathcal{P}(Y) = \text{RHS}$.

Counterexample to $\mathcal{P}(X-Y) - \{\emptyset\} = \mathcal{P}(X) - \mathcal{P}(Y)$

$Y = \{0\}$, $X = \{0, 1\}$. Then $X-Y = \{1\}$.

LHS = $\{\emptyset, \{1\}\} - \{\emptyset\} = \{\{1\}\}$.

RHS = $\{\emptyset, \{0\}, \{1\}, \{0, 1\}\} - \{\emptyset, \{0\}\}$

= $\{\{1\}, \{0, 1\}\}$. not equal.

Q4C61

Using set identities,

9

$$(A \cap (A - B)) \cup (A^c \cup B)^c \quad [\text{Set difference Law}]$$

$$= (A \cap (A \cap B^c)) \cup (A^c \cup B)^c \quad [\text{De Morgan's Law}]$$

$$= (A \cap (A \cap B^c)) \cup ((A^c)^c \cap B^c) \quad [\text{Double complement Law}]$$

$$= (A \cap (A \cap B^c)) \cup (A \cap B^c) \quad [\text{Commutative Law}]$$

$$= (A \cap B^c) \cup ((A \cap B^c) \cap A) \quad [\text{Absorption Law}]$$

$$= A \cap B^c \quad [\text{Set difference Law}]$$

$$= A - B$$

Q4(c)

By trying out a few values of x ,
it's easy to see that (i) is true, (ii) is false.

(i) By definition of $\lfloor -x \rfloor$,

$$\lfloor -x \rfloor \leq -x < \lfloor -x \rfloor + 1$$

By definition of $\lceil x \rceil$,

$$\lceil x \rceil - 1 < x \leq \lceil x \rceil$$

Adding the inequalities gives

$$\lfloor -x \rfloor + \lceil x \rceil - 1 < -x + x < \lfloor -x \rfloor + 1 + \lceil x \rceil$$

$$\underbrace{\lfloor -x \rfloor + \lceil x \rceil - 1}_{< 0} < 0 < \underbrace{\lfloor -x \rfloor + \lceil x \rceil + 1}_{> 0}$$

$$\lfloor -x \rfloor + \lceil x \rceil < 1$$

$$\lfloor -x \rfloor + \lceil x \rceil > -1$$

$$\lfloor -x \rfloor + \lceil x \rceil \leq 0$$

$$\lfloor -x \rfloor + \lceil x \rceil \geq 0$$

Since it's an integer

Since it's an integer

We conclude $\lfloor -x \rfloor + \lceil x \rceil = 0$

$$\lfloor -x \rfloor = -\lceil x \rceil$$

(ii) Take $x = \frac{1}{2}$, $\left. \begin{aligned} \lfloor -x \rfloor &= \lfloor -\frac{1}{2} \rfloor = -1 \\ -\lceil x \rceil &= -\lceil \frac{1}{2} \rceil = 0 \end{aligned} \right\} \text{ not equal.}$

Q5(a) Let $0 < x < y$. Let $n = \lceil \frac{1}{y-x} \rceil$ and $m = \lfloor ny \rfloor$.

Then n, m are integers.

By definition of $\lceil \frac{1}{y-x} \rceil$, we have $\frac{1}{y-x} \leq \lceil \frac{1}{y-x} \rceil$.

So, $1 \leq n(y-x)$ (inequality does not flip around as $y-x > 0$).

So $nx+1 \leq ny$.

By definition of $\lfloor ny \rfloor$, $m \leq ny < m+1$.

Thus, $nx \leq ny-1 < m$ and so

$$nx < m \leq ny.$$

$$nx \leq m \leq ny.$$

Q5(b) Let a be an odd integer. Then $a = 2k+1$ for

some integer k . Then $a^3 - a = a(a^2 - 1)$

$$= (2k+1)((2k+1)^2 - 1) = (2k+1)(4k^2 + 4k + 1 - 1)$$

$$= (2k+1)(4k^2 + 4k) = 8k^3 + 12k^2 + 4k$$

$$= 4k(2k^2 + 3k + 1) = 4k(2k+1)(k+1)$$

$$= 4k(k+1)(2k+1)$$

By a result in class, $k(k+1)$ is even. Let $k(k+1) = 2\ell$

So, $a^3 - a = 4(2\ell)(2k+1) = 8\ell(2k+1)$, is divisible by 8.

Alternatively, you can proceed by the following

let a be an odd integer.

Then $a = 4k+1$ or $a = 4k+3$ for some integer k .

$$\begin{aligned} \text{Case 1: } a = 4k+1. \quad a^3 - a &= (4k+1)(16k^2 + 8k + 1 - 1) \\ &= (4k+1)(16k^2 + 8k) \\ &= 8(4k+1)(2k^2 + k) \end{aligned}$$

$$\begin{aligned} \text{Case 2: } a = 4k+3. \quad a^3 - a &= (4k+3)(16k^2 + 24k + 9 - 1) \\ &= (4k+3)(16k^2 + 24k + 8) \\ &= 8(4k+3)(2k^2 + 3k + 1) \end{aligned}$$

In either case, $a^3 - a$ is divisible by 8.

Q5(c)

$$630 = 96 \times 6 + 54$$

$$96 = 54 \times 1 + 42$$

$$54 = 42 \times 1 + 12$$

$$42 = 12 \times 3 + \textcircled{6} \longrightarrow \gcd(630, 96) = 6.$$

$$12 = 6 \times 2 + 0$$

$$\boxed{Q6(a)} \quad z^3 = 3(1+i)$$

$$= 3e^{i\frac{\pi}{4}}$$

$$z = 18^{\frac{1}{6}} e^{i\frac{\frac{\pi}{4} + 2k\pi}{3}} \quad k=0, 1, 2$$

$$= 18^{\frac{1}{6}} e^{i\frac{\pi}{12}}, 18^{\frac{1}{6}} e^{i\frac{9\pi}{12}}, 18^{\frac{1}{6}} e^{i\frac{17\pi}{12}}$$

$$\boxed{Q6(b)} \quad \text{Let } g: P(\mathbb{R}) \rightarrow P(\mathbb{R}^2),$$

$$g(A) = A \times A$$

g is one-to-one: Suppose $g(A) = g(B)$.

$$A \times A = B \times B$$

Show: $A=B$: for any x , $x \in A \Leftrightarrow (x, x) \in A \times A$

$$\Leftrightarrow (x, x) \in B \times B$$

$$\Leftrightarrow x \in B.$$

g is not onto:

$$\text{Take } C = \{(0, 1)\} \in P(\mathbb{R}^2).$$

$$\text{If } g(A) = C$$

then $A \times A = \{(0, 1)\}$ So, $(0, 1) \in A \times A$.

So $0 \in A$. This means $(0, 0) \in A \times A = g(A) = C$.

Contradiction.

Q7(a) (i) A symmetric binary relation R is a relation on a set A such that for all $x, y \in A$, if $(x, y) \in R$ then $(y, x) \in R$.

(ii) A transitive binary relation R is a relation on a set A such that for every $x, y, z \in A$, if $(x, y) \in R$ and $(y, z) \in R$ then $(x, z) \in R$.

Q7(b) No it is not reflexive.

(i) $0 < 0$ is false, so $(0, 0) R (0, 0)$ is false.

(ii) No it is not symmetric.

Take $\overset{(a,b)}{(0,0)}$ and $\overset{(x,y)}{(1,0)}$.

Then $(0,0) R (1,0)$ is true as $0 < 1$

but $(1,0) R (0,0)$ is false because $1 < 0$ false and $1 = 0$ is false.

(iii) Yes it is transitive.

Fix $(a,b), (x,y), (u,v)$ such that

$(a,b) R (x,y)$ and $(x,y) R (u,v)$.

Case 1: $a < x$. Then since $(x,y) R (u,v)$ we have $x \leq u$. This means $a < x \leq u \Rightarrow a < u$.

So $(a,b) R (u,v)$ is true.

Case 2: $x < u$. Then since $(a, b) R (x, y)$,

hence $a \leq x$. So, $a \leq x < u \Rightarrow a < u$.

So again, $(a, b) R (u, v)$ true.

Case 3: $a = x$ and $x = u$: Then since $(a, b) R (x, y)$,

we have $b < y$. Since $(x, y) R (u, v)$, we

have $y < v$. So we have:

$a = x = u$ & $b < y < v$. So, $a = u$ & $b < v$.

Thus $(a, b) R (u, v)$ is true.

Q7(c) T is reflexive: 1. $a = a$ and 1. $b = b$
So, $(a, b) R (a, b)$ true.

T is symmetric. Suppose $(a, b) T (x, y)$. Let $c \neq 0$ s.t.

$ca = x$ and $cb = y$. Then $a = \frac{1}{c}x$ and $b = \frac{1}{c}y$

where $\frac{1}{c} \neq 0$. So, $(x, y) T (a, b)$ true.

T is transitive. Suppose $(a, b) T (x, y)$ and $(x, y) T (u, v)$.

Let $c \neq 0$, $d \neq 0$ s.t. $ca = x$, $cb = y$, $dx = u$, $dy = v$.

Then $dc a = dx = u$ and $dc b = dy = v$. Since $dc \neq 0$,
(by zero product property), so, $(a, b) T (u, v)$.

Equivalence class of $(1, 2)$: $(a, b) \in [(1, 2)]$

$\Leftrightarrow \exists c \neq 0$ s.t. $c \cdot 1 = a$ & $c \cdot 2 = b$

$\Leftrightarrow (a, b) = (c, 2c)$ some $c \neq 0$.

This is the line $y = 2x$ with $(0, 0)$ removed.